theories/Dot/misc/path_repl_dead.v
@@ -1,0 +1,532 @@
+From iris.proofmode Require Import tactics.
+
+From D.Dot.syn Require Import syn path_repl.
+From D.Dot.lr Require Import unary_lr path_wp path_repl.
+
+Implicit Types
+         (T : ty) (v w : vl) (t : tm) (d : dm) (ds : dms) (p q : path)
+         (Γ : ctx) (vs : vls) (l : label).
+
+Implicit Types (Pv : vl → Prop).
+Set Nested Proofs Allowed.
+
+Notation unshifts T := { T' | T = shift T' }.
+
+Lemma shift_unshift T: unshift (shift T) = T.
+Proof. by rewrite hsubst_comp hsubst_id. Qed.
+Lemma decide_unshift_proof {T} : T ≠ shift (unshift T) → unshifts T → False.
+Proof. move => Hne [T' Hn]. apply: Hne. by rewrite Hn shift_unshift. Qed.
+
+Definition decide_unshift T : unshifts T + (unshifts T → False) :=
+  match decide (T = shift (unshift T)) with
+  | left Heq => inl (unshift T ↾ Heq)
+  | right Hne => inr (decide_unshift_proof Hne)
+  end.
+Instance decision_unshift T : Decision (∃ T', T = shift T').
+Proof.
+  destruct (decide_unshift T) as [[T' Heq]|Hne]; [left|right]; naive_solver.
+Qed.
+
+(* Definition unshift_opt (T : ty) : option ty :=
+  if decide (T = (unshiftB T).|[ren (+1)])
+  then Some (unshiftB T)
+  else None. *)
+
+Section equivI_utils.
+  Context `{dlangG Σ}.
+
+  Lemma exists_equivI {A} {PROP: sbi} (φ1 φ2 : A -d> PROP) :
+    (∀ x, φ1 x ≡ φ2 x) ⊢@{PROP}
+    (∃ x, φ1 x) ≡ ∃ x, φ2 x.
+  Proof.
+    rewrite -discrete_fun_equivI.
+    apply (@f_equiv _ _ _ (λ φ : _ -d> _, ∃ x, φ x)%I). solve_proper.
+  Qed.
+
+  Lemma forall_equivI {A} {PROP: sbi} (φ1 φ2 : A -d> PROP) :
+    (∀ x, φ1 x ≡ φ2 x) ⊢@{PROP}
+    (∀ x, φ1 x) ≡ ∀ x, φ2 x.
+  Proof.
+    rewrite -discrete_fun_equivI.
+    apply (@f_equiv _ _ _ (λ φ : _ -d> _, ∀ x, φ x)%I). solve_proper.
+  Qed.
+
+  Lemma wp_equivI (φ1 φ2 : vl -d> iPropO Σ) t :
+    (∀ x, φ1 x ≡ φ2 x) ⊢@{iPropI Σ}
+    WP t {{ φ1 }} ≡ WP t {{ φ2 }}.
+  Proof.
+    rewrite -discrete_fun_equivI.
+    apply (@f_equiv _ _ _ (λ φ : _ -d> _, WP t {{ φ }})%I). solve_proper.
+  Qed.
+
+  Lemma or2_equivI {PROP : sbi} (P1 P2 Q : PROP) :
+    P1 ≡ P2 ⊢@{PROP} (P1 ∨ Q) ≡ (P2 ∨ Q).
+  Proof. apply (@f_equiv _ _ _ (λ P, P ∨ Q)%I). solve_proper. Qed.
+
+  Lemma and2_equivI {PROP : sbi} (P1 P2 Q : PROP) :
+    P1 ≡ P2 ⊢@{PROP} (P1 ∧ Q) ≡ (P2 ∧ Q).
+  Proof. apply (@f_equiv _ _ _ (λ P, P ∧ Q)%I). solve_proper. Qed.
+
+  Lemma wand2_equivI {PROP : sbi} (P1 P2 Q : PROP) :
+    P1 ≡ P2 ⊢@{PROP} (P1 -∗ Q) ≡ (P2 -∗ Q).
+  Proof. apply (@f_equiv _ _ _ (λ P, P -∗ Q)%I). solve_proper. Qed.
+End equivI_utils.
+
+Ltac iProperness :=
+  repeat first
+  [ iEval (progress rewrite -(wp_equivI, exists_equivI, forall_equivI)); iIntros
+  (* f_equiv must come before those others for performance. *)
+  | iEval (progress rewrite -(f_equiv, and2_equivI, wand2_equivI, or2_equivI))
+  ].
+
+(** Lemma [psubst_path_implies] requires [path_repl_longer], which
+requires a diversion to prove.
+I'm not sure going through sizes is the shortest proof, but that's the
+obvious way on paper, and works well in Coq too. *)
+Section psubst_path_implies_lemmas.
+  Definition append_ls p (ls : list label) : path := foldr (flip pself) p ls.
+
+  Fixpoint path_size p := match p with
+    | pv _ => 0
+    | pself p _ => 1 + path_size p
+    end.
+
+  Lemma occurs_in_path_repl {p1 p2 p q} :
+    p1 ~pp[ p := q ] p2 →
+    ∃ n, n + path_size p = path_size p1.
+  Proof.
+    elim => [|p1' p2' l Hr [n IHr]];
+      [ by exists 0 | exists (S n); by rewrite /= IHr].
+  Qed.
+
+  Lemma path_size_append p ls :
+    path_size (append_ls p ls) = length ls + path_size p.
+  Proof. by elim: ls => /= [| _ ls ->]. Qed.
+
+  Lemma path_repl_longer ls {p p1 p2 q l} :
+    p1 ~pp[ p := q ] p2 →
+    ~append_ls p1 (l :: ls) = p.
+  Proof.
+    move => /occurs_in_path_repl [ls' Hr] /(f_equal path_size).
+    rewrite /= path_size_append. lia.
+  Qed.
+End psubst_path_implies_lemmas.
+
+(** Path substitution agrees with path replacement. *)
+Lemma psubst_path_implies p1 p2 p q :
+  p1 ~pp[ p := q ] p2 →
+  p1 .p[ p := q ] = p2.
+Proof.
+  move => Hr.
+  elim: Hr => [|p1' p2' l Hr IHr] /=; first exact: psubst_path_self.
+  case_decide as Hdec => //; last by rewrite -IHr.
+  exfalso; exact: (path_repl_longer []).
+Qed.
+(**
+https://en.wikipedia.org/wiki/Idempotence#Idempotent_functions *)
+Definition IdempotentUnary {A} (f: A → A) := ∀ x, f (f x) = f x.
+
+Goal ~(∀ p q, IdempotentUnary (psubst_path p q)).
+Proof.
+  move => Hpsubst_path_idempotent.
+  set p0 := pv (ids 0).
+  move: (Hpsubst_path_idempotent p0 (pself p0 "A") p0).
+  by repeat (simplify_eq/=; case_decide).
+Qed.
+
+Lemma psubst_one_shift_id q r : shift r .p[ pv (ids 0) := q ] = shift r.
+Proof.
+  elim: r => /= [v|r -> l]; case_decide => //; destruct v; simplify_eq.
+Qed.
+
+Lemma psubst_path_pv_idempotent v q
+  (Heq : psubst_path (pv v) q q = q):
+  IdempotentUnary (psubst_path (pv v) q).
+Proof.
+  elim => [vr|r' IHq l] //=; case_decide; simplify_eq/=;
+    try case_decide; by f_equal.
+Qed.
+
+Lemma psubst_path_one_idempotent q:
+  IdempotentUnary (psubst_path (pv (ids 0)) (shift q)).
+Proof. apply psubst_path_pv_idempotent, psubst_one_shift_id. Qed.
+
+(**
+  Never even remotely true. One thing substitutes away, another substitutes
+  in the same conrtext. Pick carefully! *)
+(* Lemma equiv p q r r':
+  shift r' = psubst_path (pv (ids 0)) (shift q) r →
+  r' = psubst_path (pv (ids 0)) q r.
+Proof.
+  elim: r => /= [v|r IHr l]; case_decide.
+  (* rewrite shift_unshift. *)
+  by rewrite hsubst_comp hsubst_id. *)
+
+Lemma psubst_path_idempotent: ∀ p q,
+  psubst_path p q q = q →
+  IdempotentUnary (psubst_path p q).
+Proof.
+  move => p q Heq r.
+  elim E: r => [v|r' IHq l] //=; case_decide as Hdec0; simplify_eq/= => //;
+    case_decide as Hdec1; simplify_eq; f_equal => //.
+  rewrite Hdec1.
+  exfalso.
+  apply Hdec0. rewrite -Hdec1. f_equal. rewrite -Heq.
+Abort.
+
+Section  psubst_path_idempotent_counterexample.
+Variable l : string.
+Let q := pv (ids 0).
+Let p := pself q l.
+Let r := p.
+Let r' := pself r l.
+Ltac check := cbv; repeat (case_match; cbn); naive_solver.
+(* rewrite /r/p/q/=; repeat (case_decide; cbn); naive_solver. *)
+
+Goal q .p[ p := q ] = q.
+Proof. check. Qed.
+
+Goal pself r l ≠ p.
+Proof. check. Qed.
+Goal pself (r .p[ p := q ]) l = p.
+Proof. check. Qed.
+Goal psubst_path p q q = q.
+Proof. check. Qed.
+
+Goal (r .p[ p := q ]) .p[ p := q ] = r .p[ p := q ].
+Proof. check. Qed.
+
+Goal ~r' .p[ p := q ] .p[ p := q ] = r' .p[ p := q ].
+Proof. check. Qed.
+
+Goal ~IdempotentUnary (psubst_path p q).
+Proof. move => /(_ r'); check. Qed.
+
+Lemma not_psubst_path_idempotent: ~∀ p q,
+  psubst_path p q q = q →
+  IdempotentUnary (psubst_path p q).
+Proof. move => /(_ p q _ r'). check. Qed.
+End psubst_path_idempotent_counterexample.
+
+(* Lemma replacing_again_wont_save_you p q p1 p2:
+  p1 ≠ p2 →
+  p1 .p[ p := q ] ≠ p2 → ~ p1 ~pp[ p := q ]* p2.
+Proof.
+  move => Hne Hne2 Hr.
+  elim: Hr Hne Hne2 => [//|p1' p2' {}p2 Hh Ht IHr] Hne Hne2.
+  move: (Hh) => /psubst_path_implies Hq1.
+  simplify_eq.
+  apply IHr => //.
+  by rewrite psubst_path_idempotent.
+Qed. *)
+
+  (* inversion Hrepl as [|? q1 ? Hh Ht]; simplify_eq.
+  move: (Hh) => /psubst_path_implies Hq1.
+  inversion Ht as [|? q2 ? Hh' Ht' Heq1 Heq2]; first simplify_eq.
+  move: (Hh') => /psubst_path_implies Hq2.
+  have ?: q1 = q2. simplify_eq. by rewrite psubst_path_idempotent.
+  simplify_eq.
+
+  induction Hrepl.
+  rewrite/Decision.
+  elim => [v//| p1' p2' p3' Hrepl H IHrepl].
+  by eapply rtc_l, IHrepl; constructor.
+Admitted. *)
+
+(* Lemma psubst_path_rtc_dec p1 p2 p q :
+  Decision (p1 ~pp[ p := q ]* p2).
+Proof.
+  case: (decide (p1 = p2)) => [->|Hne]; first by left; constructor.
+  case: (decide (p1 .p[ p := q ] = p2)) => [<-|Hne2];
+    first by left; exact: psubst_path_rtc_sufficient.
+  right => Hrepl. exact: replacing_again_wont_save_you.
+Qed. *)
+
+
+Section psubst_path_implies_lemmas_extras.
+  Lemma occurs_in_path_repl_append {p1 p2 p q} :
+    p1 ~pp[ p := q ] p2 →
+    ∃ ls, append_ls p ls = p1.
+  Proof.
+    elim => [|p1' p2' l' Hr [ls' IHr]];
+      [ exists [] | exists (l' :: ls')]; by simplify_eq.
+  Qed.
+
+  Lemma paths_well_founded {ls1 ls2 p q l} :
+    append_ls q (l :: ls1) = p →
+    ~append_ls p ls2 = q.
+  Proof.
+    move => /(f_equal path_size) Heq1 /(f_equal path_size) Heq2.
+    move: Heq1 Heq2. rewrite !path_size_append /=. lia.
+  Qed.
+
+  Lemma path_repl_longer2 ls {p p1 p2 q l} :
+    p1 ~pp[ p := q ] p2 →
+    ~append_ls p1 (l :: ls) = p.
+  Proof.
+    move => /occurs_in_path_repl_append [ls' Hr] Happ.
+    exact: paths_well_founded.
+  Qed.
+End psubst_path_implies_lemmas_extras.
+
+(* Useful ???*)
+Lemma psubst_path_eq p q r: psubst_path p q r =
+  match (decide (r = p)) with
+  | left _ => q
+  | _ =>
+    match r with
+    | pv _ => r
+    | pself r' l => pself (psubst_path p q r') l
+    end
+  end.
+Proof. by case: r. Qed.
+
+(* No reason for bundling subst any more. *)
+Notation alias_paths_subst p q ρ := (alias_paths p.|[ρ] q.|[ρ]).
+
+Lemma alias_paths_weaken p q ρ v:
+  alias_paths_subst p.|[ren (+1)] q.|[ren (+1)] (v .: ρ) =
+  alias_paths_subst p q ρ.
+Proof. by rewrite !hsubst_comp ren_scons. Qed.
+
+Definition alias_pathsI {Σ} p q : iProp Σ := ⌜alias_paths p q⌝.
+Definition alias_paths_substI {Σ} p q ρ : iProp Σ := ⌜alias_paths_subst p q ρ⌝.
+Section path_repl.
+  Context `{dlangG Σ}.
+  Implicit Types (φ: vl → iProp Σ).
+
+  Notation alias_pathsI p q := (@alias_pathsI Σ p q).
+  Notation alias_paths_substI p q ρ := (@alias_paths_substI Σ p q ρ).
+(*
+  Lemma and_equivI {PROP : sbi} (P1 P2 Q1 Q2 : PROP) :
+    P1 ≡ P2 ⊢@{PROP} Q1 ≡ Q2 -∗
+    (P1 ∧ Q1) ≡ (P2 ∧ Q2).
+  Proof.
+  Admitted. *)
+
+  Lemma alias_paths_substI_symm p q :
+    alias_pathsI p q -∗ alias_pathsI q p.
+  Proof. iIntros "!%". exact: alias_paths_symm'. Qed.
+
+  Lemma alias_paths_substI_elim_eq' φ p q:
+    alias_pathsI p q ⊢
+    ⌜path_wp p φ ≡ path_wp q φ⌝.
+  Proof. iIntros "!%". apply alias_paths_elim_eq. Qed.
+
+  Lemma alias_paths_subst_elim_wand φ p q:
+    alias_paths p q →
+    path_wp p φ ⊢ path_wp q φ.
+  Proof. iIntros (->%(alias_paths_elim_eq φ)) "$". Qed.
+
+  Lemma alias_paths_subst_elim_wand' φ p q:
+    alias_pathsI p q ⊢
+    path_wp p φ -∗ path_wp q φ.
+  Proof. iIntros (->%(alias_paths_subst_elim_wand φ)) "$". Qed.
+
+  Lemma alias_paths_substI_eq p q:
+    alias_pathsI p q ⊣⊢
+    ∃ v,
+      path_wp p (λ vp : vl, ⌜v = vp⌝) ∧
+      path_wp q (λ vq : vl, ⌜v = vq⌝).
+  Proof. iIntros "!%". apply alias_paths_sameres. Qed.
+
+  Lemma alias_paths_subst_samepwp' p q:
+    alias_pathsI p q ⊣⊢
+      (∃ u, path_wp p (λ vp, ⌜u = vp⌝)) ∧
+      ∀ φ, ⌜path_wp p φ ≡ path_wp q φ⌝.
+  Proof. iIntros "!%". apply alias_paths_samepwp. Qed.
+
+
+  (** Beware: we can do path replacement *before* substitution,
+      even tho substitution and path replacement don't commute nicely.
+
+      As a special case, we get the less surprising:
+      [alias_paths_subst_pure p r ids → path_wp q φ ≡ path_wp (q .p[p := r]) φ].
+
+      But we do need the general form. *)
+  Lemma path_replacement_equiv_alt {p r ρ} q (φ : vl → iProp Σ):
+    alias_paths_subst p r ρ →
+    path_wp q.|[ρ] φ ≡ path_wp (q .p[p := r]).|[ρ] φ.
+  Proof.
+    elim: q φ => [w | q IHq l] φ /=; case_decide.
+    - simplify_eq. apply (alias_paths_elim_eq φ (pv w.[ρ]) r.|[ρ]).
+    - done.
+    - simplify_eq.
+      rewrite /= !path_wp_eq alias_paths_sameres /=.
+      destruct 1 as (vr & (vq & Hq & w & Hl & ->)%path_wp_pure_eq & Hr).
+      iSplit.
+      + iDestruct 1 as (vq' Hq' vr' Hl') "Hφ".
+        rewrite (path_wp_pure_det Hq' Hq) in Hl'.
+        objLookupDet. eauto.
+      + iDestruct 1 as (vr' Hr') "Hφ".
+        rewrite (path_wp_pure_det Hr' Hr).
+        eauto.
+    - exact: IHq.
+  Qed.
+
+  Lemma path_replacement_equiv_alt' {p r ρ} q (φ : vl → iProp Σ):
+    alias_paths_substI p r ρ ⊢
+    path_wp q.|[ρ] φ ≡ path_wp (q .p[p := r]).|[ρ] φ.
+  Proof. iIntros (?) "!%". exact: path_replacement_equiv_alt. Qed.
+
+  Lemma rewrite_tsel_psubst2 p q l ρ v r:
+    alias_paths_substI p r ρ ⊢
+    ⟦ TSel q l ⟧ ρ v ≡ ⟦ TSel (q .p[ p := r ]) l ⟧ ρ v.
+  Proof. exact: path_replacement_equiv_alt'. Qed.
+
+
+  (* That's false, as we don't know that q terminates from the hyp. *)
+  (* Lemma path_replacement_equiv_0 {p r ρ} q:
+    alias_paths_subst p r ρ ⊢@{iPropI Σ}
+    alias_paths_subst q (q .p[p := r]) ρ.
+  Proof.
+    elim: q => [w | q IHq l] /=; case_decide; simplify_eq/=.
+    - by iIntros.
+    - rewrite -alias_paths_subst_refl_vl. by iIntros.
+    - by iIntros.
+    - rewrite /= IHq !alias_paths_subst_sameres /=.
+      iDestruct 1 as (vr) "#[Hq Hqr]".
+      (* We don't know that [pself q l] terminates! *)
+  Abort. *)
+
+  (* Lemma rewrite_ty_path_repl'_slow p q T1 T2 ρ v:
+    T1 ~Tp[ p := q ] T2 →
+    ⌜alias_paths_subst_pure p q ρ⌝ ⊢@{iPropI Σ} (* p : q.type *)
+    ⟦ T1 ⟧ ρ v ≡ ⟦ T2 ⟧ ρ v.
+  Proof.
+    move => Hrew; move: v ρ.
+    induction Hrew => v ρ;
+      iIntros "/= #H"; iProperness; last
+      iApply path_replacement_equiv';
+      try by [|iApply IHHrew; rewrite ?alias_paths_subst_weaken].
+  Qed. *)
+
+
+      (* rewrite -?exists_equivI; iIntros; rewrite -?f_equiv.
+    1-2: rewrite -forall_equivI; iIntros (w).
+    by iRewrite (IHHrew w with "H").
+    rewrite -f_equiv -wp_equivI; iIntros.
+    1-2: by iApply IHHrew; rewrite // hsubst_comp subst_comp ren_scons.
+    all: rewrite -exists_equivI; iIntros (w); rewrite -!f_equiv.
+    by iRewrite (IHHrew w with "H").
+    rewrite -?and2_equivI.
+    rewrite -f_equiv.
+    all: rewrite -forall_equivI; iIntros (v0); by iRewrite (IHHrew v0 with "H").
+  Qed. *)
+      (* rewrite -f_equiv -wp_equivI; iIntros.
+
+       iApply "H".
+    (* iDestruct 1 as (t Heq) "#H1"; iExists t; iSplit; first done; iIntros "!>!>" (w) "#Ha"; *)
+      by iRewrite (IHHrew w with "H").
+      iApply internal_eq_proper. exist_proper.
+    f_equiv.
+    properness.
+    iDestruct 1 as "H1".
+    iDestruct 1 as (t Heq) "H1". iExists t; iSplit; first done; iIntros "!>!>" (w) "#Ha"; iApply "H1"; by iApply IHHrew. *)
+
+    (* move HE: (pv vr) => q Hrew.
+    iInduction Hrew as [] "IHHrew" forall (v ρ vr HE); subst q;
+      last iApply rewrite_tsel_psubst2; iIntros "/= #H";
+      try by iRewrite ("IHHrew" $! v with "[//] H").
+      try by iRewrite ("IHHrew" with "[//] H").
+       iApply prop_ext; iModIntro; iSplit. *)
+
+(* Axiom skip: forall a, a. *)
+  (* Special cases, any use? *)
+  (* Lemma path_replacement_equiv_special {p vr ρ} q (φ : vl → iProp Σ):
+    path_wp p.|[ρ] (λ w, ⌜ w = vr.[ρ] ⌝) ⊢@{iPropI Σ}
+    path_wp q.|[ρ] φ ≡ path_wp (q .p[p := pv vr]).|[ρ] φ.
+  Proof. rewrite -path_replacement_equiv' -simpl_alias_1.
+  by iIntros "!%". Qed.
+
+  Lemma rewrite_tsel_psubst2_special p q l ρ v vr:
+    path_wp p.|[ρ] (λ w, ⌜ w = vr.[ρ] ⌝) ⊢@{iPropI Σ}
+    ⟦ TSel q l ⟧ ρ v ≡ ⟦ TSel (q .p[ p := pv vr ]) l ⟧ ρ v.
+  Proof. exact: path_replacement_equiv_special. Qed. *)
+
+  (* Lemma rewrite_ty_path_repl p T1 T2 ρ v vr:
+    T1 ~Tp[ p := pv vr ] T2 →
+    path_wp p.|[ρ] (λ w, ⌜ w = vr.[ρ] ⌝) ⊢@{iPropI Σ}
+    □(⟦ T1 ⟧ ρ v ∗-∗ ⟦ T2 ⟧ ρ v).
+  Proof.
+    (* V1: gets type error at Qed, due to [dependent induction]. *)
+    intros Hrew; move: v ρ; dependent induction Hrew => v ρ;
+    (* V2 *)
+    (* move HE: (pv vr) => q; move => Hrew; move: v ρ vr HE. induction Hrew => v ρ vr HE; subst q; *)
+      last apply skip; iIntros "/= #H !>"; iSplit.
+    1-4: iIntros "[??]"; iFrame; by iApply IHHrew.
+    1-4: iIntros "[?|?]"; iFrame; by (iLeft + iRight); iApply IHHrew.
+    1-2: iIntros "? !>"; by iApply IHHrew.
+    1-2: iDestruct 1 as (t Heq) "#H1"; iExists t; iSplit; first done; iIntros "!>!>" (w) "#Ha"; iApply "H1"; by iApply IHHrew.
+    1-2: iDestruct 1 as (t Heq) "#H1"; iExists t; iSplit; first done; iIntros "!>!>" (w) "#Ha";
+      iApply (wp_wand with "(H1 Ha)").
+    1-4: iIntros; iApply IHHrew; rewrite // hsubst_comp subst_comp ren_scons; iApply "H".
+    1-2: iDestruct 1 as (d Hl vm Heq) "H1"; iExists d; iSplit; first done; iExists vm; iSplit; first done; by iApply IHHrew.
+    1-4: iDestruct 1 as (d Hl ψ) "[Hl #[HL HU]]"; iExists d; iSplit; first done; iExists ψ; iSplit; first done; iModIntro; iSplit; iIntros.
+      1-8: try ((iApply "HL" || iApply "HU"); by [iApply IHHrew|]).
+      1-2: iApply IHHrew; by [iApply "HL"|iApply "HU"|].
+  Qed. *)
+
+  (* Looks very false. *)
+  (* Lemma swap_substs p q r ρ: (q .p[ p := r ]).|[ren ρ] = q.|[ren ρ] .p[ p.|[ren ρ] := r.|[ren ρ]].
+  Proof.
+    induction q eqn:Heq; cbn; case_decide; try by simplify_eq/=; rewrite 1?decide_True.
+    case_decide => //=.
+    rewrite H1. f_equal.
+    simplify_eq/=.
+  elim: q => /= [v | q IHq l]; case_decide; simplify_eq/=; try by rewrite 1?decide_True.
+
+  rewrite decide_False; simplify_eq/=. done. naive_solver. congruence. *)
+
+  Lemma rewrite_ty_path_repl' p q T1 T2 ρ v:
+    T1 ~Tp[ p := q ] T2 →
+    alias_paths_substI p q ρ ⊢
+    ⟦ T1 ⟧ ρ v ≡ ⟦ T2 ⟧ ρ v.
+  Proof. iIntros "!%". exact: rewrite_ty_path_repl. Qed.
+
+  Lemma TMu_E_bad Γ T T' p i :
+    nclosed p (length Γ) →
+    nclosed T (1 + length Γ) →
+    T.|[ids (1 + length Γ)/] ~Tp[ pv (ids (1 + length Γ)) := p ] T' →
+    Γ ⊨p p : TMu T, i -∗ Γ ⊨p p : TMu T', i.
+  Proof.
+    intros Hclp HclT Hrepl.
+    iIntros "#Hp !>" (ρ) "Hg"; iSpecialize ("Hp" with "Hg"); iNext.
+    rewrite !path_wp_eq.
+    iDestruct "Hp" as (v Heq) "Hp"; iExists v; iFrame (Heq).
+    have Hal: alias_paths p.|[ρ] (pv v). exact Heq.
+    (* iApply interp_weaken_one. *)
+    (* rewrite interp_subst_compose_ind. asimpl. *)
+    (* Check (rewrite_ty_path_repl Hrepl). *)
+    cbn.
+    rewrite -(rewrite_ty_path_repl Hrepl).
+    rewrite interp_subst_one /=.
+    (* iApply "Hp". *)
+    asimpl.
+    (* rewrite interp_subst_one /=.
+    admit. *)
+  Abort.
+
+  Lemma TMu_E_real_bad Γ T T' p ρ v :
+    alias_paths p.|[ρ] (pv v.[ρ]) →
+    T.|[v/] ~Tp[ pv v := p ] T' →
+    path_wp p.|[ρ] (⟦ TMu T ⟧ ρ) -∗ path_wp p.|[ρ] (⟦ T' ⟧ ρ).
+  Proof.
+    intros Heq0 Hrepl.
+    rewrite !path_wp_eq.
+    iDestruct 1 as (w Heq) "Hp"; iExists w; iFrame (Heq).
+    have ?: w = v.[ρ]. exact: path_wp_pure_det.
+    subst.
+    have Hal: alias_paths p.|[ρ] (pv v.[ρ]). apply Heq.
+    (* have Hal2: alias_paths p.|[ρ] (pv v).|[ρ]. admit. *)
+    (* cbn. iPoseProof (rewrite_ty_path_repl with "Hp") as "Hp'". *)
+    iApply (rewrite_ty_path_repl Hrepl).
+    exact: alias_paths_symm'.
+    by rewrite interp_subst_one.
+  Qed.
+
+  Let Ts := TAnd (TAnd (TSel (pv (ids 0)) "A") (TSel (pv (ids 1)) "B"))
+      (TSel (pv (ids 2)) "B").
+  Let HclTs : nclosed Ts 3. solve_fv_congruence. Qed.
+  (* Eval cbv in Ts.|[ids (1 + 1)/]. *)
+End path_repl.
