theories/Dot/syn/path_repl.v
@@ -1,0 +1,205 @@
+From D.Dot.syn Require Import syn.
+Implicit Types
+         (T : ty) (v w : vl) (t : tm) (d : dm) (ds : dms) (p q : path)
+         (l : label).
+
+Notation shift T := T.|[ren (+1)].
+Notation unshift T := T.|[ren pred].
+
+Reserved Notation "p1 ~pp[ p := q  ] p2" (at level 70).
+Inductive path_path_repl (p q : path) : path → path → Prop :=
+| path_path_repl_base : p ~pp[ p := q ] q
+| path_path_repl_self p1 p2 l :
+  p1 ~pp[ p := q ] p2 →
+  pself p1 l ~pp[ p := q ] pself p2 l
+where "p1 ~pp[ p := q  ] p2" := (path_path_repl p q p1 p2) .
+
+Lemma path_path_repl_id p1 p2 p : p1 ~pp[ p := p ] p2 → p1 = p2.
+Proof. by elim; intros; simplify_eq/=. Qed.
+
+Notation path_path_repl_rtc p q := (rtc (path_path_repl p q)).
+Notation "p1 ~pp[ p := q  ]* p2" := (path_path_repl_rtc p q p1 p2) (at level 70).
+
+Reserved Notation "T1 ~Tp[ p := q  ] T2" (at level 70).
+
+(** The path replacement judgment, as defined in the pDOT paper. *)
+(*
+  This does only one replacement, as path replacement in the pDOT paper.
+  Path substitution is a particular sequene of such replacements, but if q contains p,
+  there are sequences of replacements that don't correspond to a single path substitution,
+  but to iterated path substitutions.
+  Nevertheless, as long as both p and q are valid in the same scope, both
+  are fine.
+  However, substitution can be sound in contexts where path replacements aren't sound.
+
+  Still, psubst_one uses path replacement with *disjoints* paths!
+*)
+Inductive ty_path_repl (p q : path) : ty → ty → Prop :=
+| ty_path_repl_TAnd1 T1 T2 U :
+  T1 ~Tp[ p := q ] T2 →
+  TAnd T1 U ~Tp[ p := q ] TAnd T2 U
+| ty_path_repl_TAnd2 T1 T2 U :
+  T1 ~Tp[ p := q ] T2 →
+  TAnd U T1 ~Tp[ p := q ] TAnd U T2
+| ty_path_repl_TOr1 T1 T2 U :
+  T1 ~Tp[ p := q ] T2 →
+  TOr T1 U ~Tp[ p := q ] TOr T2 U
+| ty_path_repl_TOr2 T1 T2 U :
+  T1 ~Tp[ p := q ] T2 →
+  TOr U T1 ~Tp[ p := q ] TOr U T2
+| ty_path_repl_TLater T1 T2 :
+  T1 ~Tp[ p := q ] T2 →
+  TLater T1 ~Tp[ p := q ] TLater T2
+| ty_path_repl_TAll1 T1 T2 U :
+  T1 ~Tp[ p := q ] T2 →
+  TAll T1 U ~Tp[ p := q ] TAll T2 U
+| ty_path_repl_TAll2 T1 T2 U :
+  T1 ~Tp[ shift p := shift q ] T2 →
+  TAll U T1 ~Tp[ p := q ] TAll U T2
+| ty_path_repl_TMu T1 T2 :
+  T1 ~Tp[ shift p := shift q ] T2 →
+  TMu T1 ~Tp[ p := q ] TMu T2
+| ty_path_repl_TVMem T1 T2 l :
+  T1 ~Tp[ p := q ] T2 →
+  TVMem l T1 ~Tp[ p := q ] TVMem l T2
+| ty_path_repl_TTMem1 T1 T2 U l :
+  T1 ~Tp[ p := q ] T2 →
+  TTMem l T1 U ~Tp[ p := q ] TTMem l T2 U
+| ty_path_repl_TTMem2 T1 T2 U l :
+  T1 ~Tp[ p := q ] T2 →
+  TTMem l U T1 ~Tp[ p := q ] TTMem l U T2
+| ty_path_repl_TSel p1 p2 l :
+  p1 ~pp[ p := q ] p2 →
+  TSel p1 l ~Tp[ p := q ] TSel p2 l
+| ty_path_repl_TSing p1 p2 :
+  p1 ~pp[ p := q ] p2 →
+  TSing p1 ~Tp[ p := q ] TSing p2
+where "T1 ~Tp[ p := q  ] T2" := (ty_path_repl p q T1 T2).
+
+Notation ty_path_repl_rtc p q := (rtc (ty_path_repl p q)).
+Notation "T1 ~Tp[ p := q  ]* T2" := (ty_path_repl_rtc p q T1 T2) (at level 70).
+
+Lemma ty_path_repl_id p T1 T2 : T1 ~Tp[ p := p ] T2 → T1 = T2.
+Proof.
+  intros Hr; dependent induction Hr; rewrite ?IHHr //;
+    f_equiv; exact: path_path_repl_id.
+Qed.
+
+(** Define substitution of [pv (ids 0)] by [p] in terms of the
+    transitive closure of path replacement.
+    Here it's crucial to use the transitive closure of path replacement
+    to substitute all occurrences. *)
+Definition psubst_one T p T' :=
+  T ~Tp[ pv (ids 0) := shift p ]* shift T'.
+Notation "T .Tp[ p /]~ T'" := (psubst_one T p T') (at level 65).
+
+Reserved Notation "r .p[ p := q  ]" (at level 65).
+Fixpoint psubst_path p q r : path := match (decide (r = p)) with
+| left _ => q
+| _ =>
+  match r with
+  | pv _ => r (* XXX no, values can contain paths! OTOH, pDOT path replacement doesn't do this. *)
+  | pself r' l => pself (r' .p[ p := q ]) l
+  end
+end
+where "r .p[ p := q  ]" := (psubst_path p q r).
+
+Lemma psubst_path_id p q : q .p[ p := p ] = q.
+Proof. elim: q => /= *; case_decide; by f_equal. Qed.
+
+Lemma psubst_path_self p q: p .p[ p := q ] = q.
+Proof. case: p => /= *; by rewrite decide_True. Qed.
+
+Reserved Notation "T .T[ p := q  ]" (at level 65).
+Fixpoint psubst_ty p q T : ty := match T with
+| TTop => TTop
+| TBot => TBot
+| TAnd T1 T2 => TAnd (T1 .T[ p := q ]) (T2 .T[ p := q ])
+| TOr T1 T2 => TOr (T1 .T[ p := q ]) (T2 .T[ p := q ])
+| TLater T1 => TLater (T1 .T[ p := q ])
+| TAll T1 T2 => TAll (T1 .T[ p := q ]) (T2 .T[ shift p := shift q ])
+| TMu T1 => TMu (T1 .T[ shift p := shift q ])
+| TVMem l T1 => TVMem l (T1 .T[ p := q ])
+| TTMem l T1 T2 => TTMem l (T1 .T[ p := q ]) (T2 .T[ p := q ])
+| TSel r l => TSel (r .p[ p := q ]) l
+| TNat => TNat
+| TSing r => TSing (r .p[ p := q ])
+end
+where "T .T[ p := q  ]" := (psubst_ty p q T).
+
+Section decide_psubst.
+  Local Hint Constructors rtc path_path_repl ty_path_repl : core.
+
+  Lemma path_path_repl_self_rtc p q p1 p2 l :
+    p1 ~pp[ p := q ]* p2 →
+    pself p1 l ~pp[ p := q ]* pself p2 l.
+  Proof. induction 1; eauto. Qed.
+
+  (** The Kleene start of path replacement agrees with path substitution.
+    In fact, there can be only 0 or 1 steps anyway. *)
+  Lemma psubst_path_rtc_sufficient p1 q1 p q :
+    p1 .p[ p := q ] = q1 →
+    p1 ~pp[ p := q ]* q1.
+  Proof.
+    move => <- {q1}.
+    elim: p1 => [v|p1 IHp1 l] /=; case_decide as Hdec;
+      [|done| |exact: path_path_repl_self_rtc];
+    rewrite Hdec; apply rtc_once; constructor.
+  Qed.
+
+  Lemma ty_path_repl_TAnd_rtc T1 T2 U1 U2 p q :
+    T1 ~Tp[ p := q ]* U1 → T2 ~Tp[ p := q ]* U2 →
+    TAnd T1 T2 ~Tp[ p := q ]* TAnd U1 U2.
+  Proof. induction 1; induction 1; eauto. Qed.
+
+  Lemma ty_path_repl_TOr_rtc T1 T2 U1 U2 p q :
+    T1 ~Tp[ p := q ]* U1 → T2 ~Tp[ p := q ]* U2 →
+    TOr T1 T2 ~Tp[ p := q ]* TOr U1 U2.
+  Proof. induction 1; induction 1; eauto. Qed.
+
+  Lemma ty_path_repl_TLater_rtc T1 U1 p q :
+    T1 ~Tp[ p := q ]* U1 →
+    TLater T1 ~Tp[ p := q ]* TLater U1.
+  Proof. induction 1; eauto. Qed.
+
+  Lemma ty_path_repl_TAll_rtc T1 T2 U1 U2 p q :
+    T1 ~Tp[ p := q ]* U1 → T2 ~Tp[ shift p := shift q ]* U2 →
+    TAll T1 T2 ~Tp[ p := q ]* TAll U1 U2.
+  Proof. induction 1; induction 1; eauto. Qed.
+
+  Lemma ty_path_repl_TMu_rtc T1 U1 p q :
+    T1 ~Tp[ shift p := shift q ]* U1 →
+    TMu T1 ~Tp[ p := q ]* TMu U1.
+  Proof. induction 1; eauto. Qed.
+
+  Lemma ty_path_repl_TVMem_rtc T1 U1 p q l :
+    T1 ~Tp[ p := q ]* U1 →
+    TVMem l T1 ~Tp[ p := q ]* TVMem l U1.
+  Proof. induction 1; eauto. Qed.
+
+  Lemma ty_path_repl_TTMem_rtc T1 T2 U1 U2 p q l :
+    T1 ~Tp[ p := q ]* U1 → T2 ~Tp[ p := q ]* U2 →
+    TTMem l T1 T2 ~Tp[ p := q ]* TTMem l U1 U2.
+  Proof. induction 1; induction 1; eauto. Qed.
+
+  Lemma ty_path_repl_TSel_rtc p1 q1 p q l :
+    p1 ~pp[ p := q ]* q1 →
+    TSel p1 l ~Tp[ p := q ]* TSel q1 l.
+  Proof. induction 1; eauto. Qed.
+
+  Lemma ty_path_repl_TSing_rtc p1 q1 p q :
+    p1 ~pp[ p := q ]* q1 →
+    TSing p1 ~Tp[ p := q ]* TSing q1.
+  Proof. induction 1; eauto. Qed.
+
+  Lemma psubst_ty_rtc_sufficient T1 T2 p q :
+    T1 .T[ p := q ] = T2 →
+    T1 ~Tp[ p := q ]* T2.
+  Proof.
+    move => <- {T2}; move: p q.
+    induction T1; eauto using ty_path_repl_TAnd_rtc, ty_path_repl_TOr_rtc,
+      ty_path_repl_TLater_rtc, ty_path_repl_TAll_rtc, ty_path_repl_TMu_rtc,
+      ty_path_repl_TTMem_rtc, ty_path_repl_TVMem_rtc, ty_path_repl_TSel_rtc,
+      ty_path_repl_TSing_rtc, psubst_path_rtc_sufficient.
+  Qed.
+End decide_psubst.
